Slightly better compilation story for read_fblock

src/BlockPtr.v
@@ -3407,7 +3407,8 @@ Module BlockPtr (BPtr : BlockPtrSig).
   (************* program *)
 
   Definition get lxp (ir : irec) off ms :=
-    If (lt_dec off NDirect) {
+    t0 <- Rdtsc;
+    r <- (If (lt_dec off NDirect) {
       Ret ^(ms, selN (IRBlocks ir) off $0)
     } else {
       let off := off - NDirect in
@@ -3422,7 +3423,10 @@ Module BlockPtr (BPtr : BlockPtrSig).
           indget 2 lxp (IRTindPtr ir) off ms
         }
       }
-    }.
+        });
+    t1 <- Rdtsc;
+    _ <- Debug "Ind.get" (t1-t0);
+  Ret r.
 
   Definition read lxp (ir : irec) ms :=
     If (le_dec (IRLen ir) NDirect) {
